Relativize axioms in recursor

operations/Recursor.thy
@@ -34,32 +34,41 @@ consts U2ctor :: "('var::{var_T1_pre,var_T2_pre}, 'tyvar::{var_T1_pre,var_T2_pre
   ('var, 'tyvar, 'a, 'b) T2 \<times> (('var, 'tyvar) P \<Rightarrow> ('var, 'tyvar, 'a, 'b) U2)
 ) T2_pre \<Rightarrow> ('var, 'tyvar) P \<Rightarrow> ('var, 'tyvar, 'a, 'b) U2"
 
+consts validP :: "('var, 'tyvar) P \<Rightarrow> bool"
+consts validU1 :: "('var, 'tyvar, 'a, 'b) U1 \<Rightarrow> bool"
+consts validU2 :: "('var, 'tyvar, 'a, 'b) U2 \<Rightarrow> bool"
+
 axiomatization where
   (* parameter axioms *)
-  Pmap_id0: "Pmap id id = id"
-  and Pmap_comp0: "bij f1 \<Longrightarrow> |supp (f1::'var::{var_T1_pre,var_T2_pre} \<Rightarrow> 'var)| <o |UNIV::'var set| \<Longrightarrow> bij f2 \<Longrightarrow> |supp (f2::'tyvar::{var_T1_pre,var_T2_pre} \<Rightarrow> 'tyvar)| <o |UNIV::'tyvar set| \<Longrightarrow>
+  Pmap_id0: "validP d \<Longrightarrow> Pmap id id d = d"
+  and Pmap_comp0: "validP d \<Longrightarrow> bij f1 \<Longrightarrow> |supp (f1::'var::{var_T1_pre,var_T2_pre} \<Rightarrow> 'var)| <o |UNIV::'var set| \<Longrightarrow> bij f2 \<Longrightarrow> |supp (f2::'tyvar::{var_T1_pre,var_T2_pre} \<Rightarrow> 'tyvar)| <o |UNIV::'tyvar set| \<Longrightarrow>
   bij g1 \<Longrightarrow> |supp (g1::'var \<Rightarrow> 'var)| <o |UNIV::'var set| \<Longrightarrow> bij g2 \<Longrightarrow> |supp (g2::'tyvar \<Rightarrow> 'tyvar)| <o |UNIV::'tyvar set| \<Longrightarrow>
-  Pmap (g1 \<circ> f1) (g2 \<circ> f2) = Pmap g1 g2 \<circ> Pmap f1 f2"
-  and Pmap_cong_id: "bij f1 \<Longrightarrow> |supp (f1::'var::{var_T1_pre,var_T2_pre} \<Rightarrow> 'var)| <o |UNIV::'var set| \<Longrightarrow> bij f2 \<Longrightarrow> |supp (f2::'tyvar::{var_T1_pre,var_T2_pre} \<Rightarrow> 'tyvar)| <o |UNIV::'tyvar set| \<Longrightarrow>
+  Pmap (g1 \<circ> f1) (g2 \<circ> f2) d = (Pmap g1 g2 \<circ> Pmap f1 f2) d"
+  and Pmap_cong_id: "validP d \<Longrightarrow> bij f1 \<Longrightarrow> |supp (f1::'var::{var_T1_pre,var_T2_pre} \<Rightarrow> 'var)| <o |UNIV::'var set| \<Longrightarrow> bij f2 \<Longrightarrow> |supp (f2::'tyvar::{var_T1_pre,var_T2_pre} \<Rightarrow> 'tyvar)| <o |UNIV::'tyvar set| \<Longrightarrow>
   (\<And>a. a \<in> PFVars_1 d \<Longrightarrow> f1 a = a) \<Longrightarrow> (\<And>a. a \<in> PFVars_2 d \<Longrightarrow> f2 a = a) \<Longrightarrow>
   Pmap f1 f2 d = d"
-  and PFVars_Pmap_1: "bij f1 \<Longrightarrow> |supp (f1::'var::{var_T1_pre,var_T2_pre} \<Rightarrow> 'var)| <o |UNIV::'var set| \<Longrightarrow> bij f2 \<Longrightarrow> |supp (f2::'tyvar::{var_T1_pre,var_T2_pre} \<Rightarrow> 'tyvar)| <o |UNIV::'tyvar set| \<Longrightarrow>
+  and PFVars_Pmap_1: "validP d \<Longrightarrow> bij f1 \<Longrightarrow> |supp (f1::'var::{var_T1_pre,var_T2_pre} \<Rightarrow> 'var)| <o |UNIV::'var set| \<Longrightarrow> bij f2 \<Longrightarrow> |supp (f2::'tyvar::{var_T1_pre,var_T2_pre} \<Rightarrow> 'tyvar)| <o |UNIV::'tyvar set| \<Longrightarrow>
   PFVars_1 (Pmap f1 f2 d) = f1 ` PFVars_1 d"
-  and PFVars_Pmap_2: "bij f1 \<Longrightarrow> |supp (f1::'var::{var_T1_pre,var_T2_pre} \<Rightarrow> 'var)| <o |UNIV::'var set| \<Longrightarrow> bij f2 \<Longrightarrow> |supp (f2::'tyvar::{var_T1_pre,var_T2_pre} \<Rightarrow> 'tyvar)| <o |UNIV::'tyvar set| \<Longrightarrow>
+  and PFVars_Pmap_2: "validP d \<Longrightarrow> bij f1 \<Longrightarrow> |supp (f1::'var::{var_T1_pre,var_T2_pre} \<Rightarrow> 'var)| <o |UNIV::'var set| \<Longrightarrow> bij f2 \<Longrightarrow> |supp (f2::'tyvar::{var_T1_pre,var_T2_pre} \<Rightarrow> 'tyvar)| <o |UNIV::'tyvar set| \<Longrightarrow>
   PFVars_2 (Pmap f1 f2 d) = f2 ` PFVars_2 d"
-  and small_PFVars_1: "|PFVars_1 d| <o |UNIV::'var set|"
-  and small_PFVars_2: "|PFVars_2 d| <o |UNIV::'tyvar set|"
+  and small_PFVars_1: "validP d \<Longrightarrow> |PFVars_1 d| <o |UNIV::'var set|"
+  and small_PFVars_2: "validP d \<Longrightarrow> |PFVars_2 d| <o |UNIV::'tyvar set|"
   and small_avoiding_set1: "|avoiding_set1::'var set| <o |UNIV::'var set|"
   and small_avoiding_set2: "|avoiding_set2::'tyvar set| <o |UNIV::'tyvar set|"
+  (* closure of validP under Pmap *)
+  and valid_Pmap: "validP d \<Longrightarrow> bij f1 \<Longrightarrow> |supp (f1::'var::{var_T1_pre,var_T2_pre} \<Rightarrow> 'var)| <o |UNIV::'var set| \<Longrightarrow> bij f2 \<Longrightarrow> |supp (f2::'tyvar::{var_T1_pre,var_T2_pre} \<Rightarrow> 'tyvar)| <o |UNIV::'tyvar set| \<Longrightarrow>
+                  validP (Pmap f1 f2 d)"
   (* model 1 axioms *)
-  and U1map_id0: "U1map id id (t1::('var, 'tyvar, 'a, 'b) T1) = id"
-  and U1map_comp0: "bij f1 \<Longrightarrow> |supp (f1::'var::{var_T1_pre,var_T2_pre} \<Rightarrow> 'var)| <o |UNIV::'var set| \<Longrightarrow> bij f2 \<Longrightarrow> |supp (f2::'tyvar::{var_T1_pre,var_T2_pre} \<Rightarrow> 'tyvar)| <o |UNIV::'tyvar set| \<Longrightarrow>
+  and U1map_id0: "validU1 u1 \<Longrightarrow> U1map id id (t1::('var, 'tyvar, 'a, 'b) T1) u1 = u1"
+  and U1map_comp0: "validU1 u1 \<Longrightarrow> bij f1 \<Longrightarrow> |supp (f1::'var::{var_T1_pre,var_T2_pre} \<Rightarrow> 'var)| <o |UNIV::'var set| \<Longrightarrow> bij f2 \<Longrightarrow> |supp (f2::'tyvar::{var_T1_pre,var_T2_pre} \<Rightarrow> 'tyvar)| <o |UNIV::'tyvar set| \<Longrightarrow>
   bij g1 \<Longrightarrow> |supp (g1::'var \<Rightarrow> 'var)| <o |UNIV::'var set| \<Longrightarrow> bij g2 \<Longrightarrow> |supp (g2::'tyvar \<Rightarrow> 'tyvar)| <o |UNIV::'tyvar set| \<Longrightarrow>
-  U1map (g1 \<circ> f1) (g2 \<circ> f2) t1 = U1map g1 g2 t1 \<circ> U1map f1 f2 t1"
-  and U1map_cong_id: "bij f1 \<Longrightarrow> |supp (f1::'var::{var_T1_pre,var_T2_pre} \<Rightarrow> 'var)| <o |UNIV::'var set| \<Longrightarrow> bij f2 \<Longrightarrow> |supp (f2::'tyvar::{var_T1_pre,var_T2_pre} \<Rightarrow> 'tyvar)| <o |UNIV::'tyvar set| \<Longrightarrow>
+  U1map (g1 \<circ> f1) (g2 \<circ> f2) t1 x1 = (U1map g1 g2 t1 \<circ> U1map f1 f2 t1) u1"
+  and U1map_cong_id: "validU1 u1 \<Longrightarrow> bij f1 \<Longrightarrow> |supp (f1::'var::{var_T1_pre,var_T2_pre} \<Rightarrow> 'var)| <o |UNIV::'var set| \<Longrightarrow> bij f2 \<Longrightarrow> |supp (f2::'tyvar::{var_T1_pre,var_T2_pre} \<Rightarrow> 'tyvar)| <o |UNIV::'tyvar set| \<Longrightarrow>
   (\<And>a. a \<in> U1FVars_1 t1 u1 \<Longrightarrow> f1 a = a) \<Longrightarrow> (\<And>a. a \<in> U1FVars_2 t1 u1 \<Longrightarrow> f2 a = a) \<Longrightarrow>
   U1map f1 f2 t1 u1 = u1"
-  and U1map_Uctor: "bij f1 \<Longrightarrow> |supp (f1::'var::{var_T1_pre,var_T2_pre} \<Rightarrow> 'var)| <o |UNIV::'var set| \<Longrightarrow> bij f2 \<Longrightarrow> |supp (f2::'tyvar::{var_T1_pre,var_T2_pre} \<Rightarrow> 'tyvar)| <o |UNIV::'tyvar set| \<Longrightarrow>
+  and U1map_Uctor: "validP p \<Longrightarrow>
+    pred_T1_pre (\<lambda>_. True) (pred_fun validP validU1 \<circ> snd) (pred_fun validP validU1 \<circ> snd) (pred_fun validP validU2 \<circ> snd) (pred_fun validP validU2 \<circ> snd) y \<Longrightarrow>
+   bij f1 \<Longrightarrow> |supp (f1::'var::{var_T1_pre,var_T2_pre} \<Rightarrow> 'var)| <o |UNIV::'var set| \<Longrightarrow> bij f2 \<Longrightarrow> |supp (f2::'tyvar::{var_T1_pre,var_T2_pre} \<Rightarrow> 'tyvar)| <o |UNIV::'tyvar set| \<Longrightarrow>
   U1map f1 f2 (T1_ctor (map_T1_pre id id id id id id fst fst fst fst y)) (U1ctor y p)
 = U1ctor (map_T1_pre f1 f2 id id f1 f2
     (\<lambda>(t, pu). (rrename_T1 f1 f2 t, \<lambda>p. U1map f1 f2 t (pu (Pmap (inv f1) (inv f2) p))))
@@ -67,23 +76,33 @@ axiomatization where
     (\<lambda>(t, pu). (rrename_T2 f1 f2 t, \<lambda>p. U2map f1 f2 t (pu (Pmap (inv f1) (inv f2) p))))
     (\<lambda>(t, pu). (rrename_T2 f1 f2 t, \<lambda>p. U2map f1 f2 t (pu (Pmap (inv f1) (inv f2) p))))
  y) (Pmap f1 f2 p)"
-  and U1FVars_subset_1: "set5_T1_pre (y::(_, _, 'a::{var_T1_pre,var_T2_pre}, 'b, _, _, _, _, _, _) T1_pre) \<inter> (PFVars_1 p \<union> avoiding_set1) = {} \<Longrightarrow>
+  and U1FVars_subset_1: "validP p \<Longrightarrow>
+  pred_T1_pre (\<lambda>_. True) (pred_fun validP validU1 \<circ> snd) (pred_fun validP validU1 \<circ> snd) (pred_fun validP validU2 \<circ> snd) (pred_fun validP validU2 \<circ> snd) y \<Longrightarrow>
+  set5_T1_pre (y::(_, _, 'a::{var_T1_pre,var_T2_pre}, 'b, _, _, _, _, _, _) T1_pre) \<inter> (PFVars_1 p \<union> avoiding_set1) = {} \<Longrightarrow>
   (\<And>t pu p. (t, pu) \<in> set7_T1_pre y \<union> set8_T1_pre y \<Longrightarrow> U1FVars_1 t (pu p) \<subseteq> FFVars_T11 t \<union> PFVars_1 p \<union> avoiding_set1) \<Longrightarrow>
   (\<And>t pu p. (t, pu) \<in> set9_T1_pre y \<union> set10_T1_pre y \<Longrightarrow> U2FVars_1 t (pu p) \<subseteq> FFVars_T21 t \<union> PFVars_1 p \<union> avoiding_set1) \<Longrightarrow>
   U1FVars_1 (T1_ctor (map_T1_pre id id id id id id fst fst fst fst y)) (U1ctor y p) \<subseteq> FFVars_T11 (T1_ctor (map_T1_pre id id id id id id fst fst fst fst y)) \<union> PFVars_1 p \<union> avoiding_set1"
-  and U1FVars_subset_2: "set6_T1_pre (y::(_, _, 'a::{var_T1_pre,var_T2_pre}, 'b, _, _, _, _, _, _) T1_pre) \<inter> (PFVars_2 p \<union> avoiding_set2) = {} \<Longrightarrow>
+  and U1FVars_subset_2: "validP p \<Longrightarrow>
+  pred_T1_pre (\<lambda>_. True) (pred_fun validP validU1 \<circ> snd) (pred_fun validP validU1 \<circ> snd) (pred_fun validP validU2 \<circ> snd) (pred_fun validP validU2 \<circ> snd) y \<Longrightarrow>set6_T1_pre (y::(_, _, 'a::{var_T1_pre,var_T2_pre}, 'b, _, _, _, _, _, _) T1_pre) \<inter> (PFVars_2 p \<union> avoiding_set2) = {} \<Longrightarrow>
   (\<And>t pu p. (t, pu) \<in> set7_T1_pre y \<union> set8_T1_pre y \<Longrightarrow> U1FVars_2 t (pu p) \<subseteq> FFVars_T12 t \<union> PFVars_2 p \<union> avoiding_set2) \<Longrightarrow>
   (\<And>t pu p. (t, pu) \<in> set9_T1_pre y \<union> set10_T1_pre y \<Longrightarrow> U2FVars_2 t (pu p) \<subseteq> FFVars_T22 t \<union> PFVars_2 p \<union> avoiding_set2) \<Longrightarrow>
   U1FVars_2 (T1_ctor (map_T1_pre id id id id id id fst fst fst fst y)) (U1ctor y p) \<subseteq> FFVars_T12 (T1_ctor (map_T1_pre id id id id id id fst fst fst fst y)) \<union> PFVars_2 p \<union> avoiding_set2"
+  (* closure of validU1 under Umap and Uctor *)
+  and validU1_Umap: "validU1 u1 \<Longrightarrow> bij f1 \<Longrightarrow> |supp (f1::'var::{var_T1_pre,var_T2_pre} \<Rightarrow> 'var)| <o |UNIV::'var set| \<Longrightarrow> bij f2 \<Longrightarrow> |supp (f2::'tyvar::{var_T1_pre,var_T2_pre} \<Rightarrow> 'tyvar)| <o |UNIV::'tyvar set| \<Longrightarrow>
+                     validU1 (U1map f1 f2  (t1::('var, 'tyvar, 'a, 'b) T1) u1)"
+  and validU1_Uctor: "pred_T1_pre (\<lambda>_. True) (pred_fun validP validU1 \<circ> snd) (pred_fun validP validU1 \<circ> snd) (pred_fun validP validU2 \<circ> snd) (pred_fun validP validU2 \<circ> snd) y
+        \<Longrightarrow> validP p \<Longrightarrow> validU1 (U1ctor y p)"
   (* model 2 axioms *)
-  and U2map_id0: "U2map id id (t2::('var, 'tyvar, 'a, 'b) T2) = id"
-  and U2map_comp0: "bij f1 \<Longrightarrow> |supp (f1::'var \<Rightarrow> 'var)| <o |UNIV::'var set| \<Longrightarrow> bij f2 \<Longrightarrow> |supp (f2::'tyvar \<Rightarrow> 'tyvar)| <o |UNIV::'tyvar set| \<Longrightarrow>
+  and U2map_id0: "validU2 u2 \<Longrightarrow> U2map id id (t2::('var, 'tyvar, 'a, 'b) T2) u2 = u2"
+  and U2map_comp0: "validU2 u2 \<Longrightarrow> bij f1 \<Longrightarrow> |supp (f1::'var \<Rightarrow> 'var)| <o |UNIV::'var set| \<Longrightarrow> bij f2 \<Longrightarrow> |supp (f2::'tyvar \<Rightarrow> 'tyvar)| <o |UNIV::'tyvar set| \<Longrightarrow>
   bij g1 \<Longrightarrow> |supp (g1::'var \<Rightarrow> 'var)| <o |UNIV::'var set| \<Longrightarrow> bij g2 \<Longrightarrow> |supp (g2::'tyvar \<Rightarrow> 'tyvar)| <o |UNIV::'tyvar set| \<Longrightarrow>
-  U2map (g1 \<circ> f1) (g2 \<circ> f2) t2 = U2map g1 g2 t2 \<circ> U2map f1 f2 t2"
-  and U2map_cong_id: "bij f1 \<Longrightarrow> |supp (f1::'var \<Rightarrow> 'var)| <o |UNIV::'var set| \<Longrightarrow> bij f2 \<Longrightarrow> |supp (f2::'tyvar \<Rightarrow> 'tyvar)| <o |UNIV::'tyvar set| \<Longrightarrow>
+  U2map (g1 \<circ> f1) (g2 \<circ> f2) t2 u2 = (U2map g1 g2 t2 \<circ> U2map f1 f2 t2) u2"
+  and U2map_cong_id: "validU2 u2 \<Longrightarrow> bij f1 \<Longrightarrow> |supp (f1::'var \<Rightarrow> 'var)| <o |UNIV::'var set| \<Longrightarrow> bij f2 \<Longrightarrow> |supp (f2::'tyvar \<Rightarrow> 'tyvar)| <o |UNIV::'tyvar set| \<Longrightarrow>
   (\<And>a. a \<in> U2FVars_1 t2 u2 \<Longrightarrow> f1 a = a) \<Longrightarrow> (\<And>a. a \<in> U2FVars_2 t2 u2 \<Longrightarrow> f2 a = a) \<Longrightarrow>
   U2map f1 f2 t2 u2 = u2"
-  and U2map_Uctor: "bij f1 \<Longrightarrow> |supp (f1::'var \<Rightarrow> 'var)| <o |UNIV::'var set| \<Longrightarrow> bij f2 \<Longrightarrow> |supp (f2::'tyvar \<Rightarrow> 'tyvar)| <o |UNIV::'tyvar set| \<Longrightarrow>
+  and U2map_Uctor: "validP p \<Longrightarrow>
+  pred_T2_pre (\<lambda>_. True) (pred_fun validP validU1 \<circ> snd) (pred_fun validP validU1 \<circ> snd) (pred_fun validP validU2 \<circ> snd) (pred_fun validP validU2 \<circ> snd) y2 \<Longrightarrow>
+  bij f1 \<Longrightarrow> |supp (f1::'var \<Rightarrow> 'var)| <o |UNIV::'var set| \<Longrightarrow> bij f2 \<Longrightarrow> |supp (f2::'tyvar \<Rightarrow> 'tyvar)| <o |UNIV::'tyvar set| \<Longrightarrow>
   U2map f1 f2 (T2_ctor (map_T2_pre id id id id id id fst fst fst fst y2)) (U2ctor y2 p)
 = U2ctor (map_T2_pre f1 f2 id id f1 f2
     (\<lambda>(t, pu). (rrename_T1 f1 f2 t, \<lambda>p. U1map f1 f2 t (pu (Pmap (inv f1) (inv f2) p))))
@@ -91,14 +110,21 @@ axiomatization where
     (\<lambda>(t, pu). (rrename_T2 f1 f2 t, \<lambda>p. U2map f1 f2 t (pu (Pmap (inv f1) (inv f2) p))))
     (\<lambda>(t, pu). (rrename_T2 f1 f2 t, \<lambda>p. U2map f1 f2 t (pu (Pmap (inv f1) (inv f2) p))))
  y2) (Pmap f1 f2 p)"
-  and U2FVars_subset_1: "set5_T2_pre (y2::(_, _, 'a, 'b, _, _, _, _, _, _) T2_pre) \<inter> (PFVars_1 p \<union> avoiding_set1) = {} \<Longrightarrow>
+  and U2FVars_subset_1: "validP p \<Longrightarrow>
+  pred_T2_pre (\<lambda>_. True) (pred_fun validP validU1 \<circ> snd) (pred_fun validP validU1 \<circ> snd) (pred_fun validP validU2 \<circ> snd) (pred_fun validP validU2 \<circ> snd) y2 \<Longrightarrow>set5_T2_pre (y2::(_, _, 'a, 'b, _, _, _, _, _, _) T2_pre) \<inter> (PFVars_1 p \<union> avoiding_set1) = {} \<Longrightarrow>
   (\<And>t pu p. (t, pu) \<in> set7_T2_pre y2 \<union> set8_T2_pre y2 \<Longrightarrow> U1FVars_1 t (pu p) \<subseteq> FFVars_T11 t \<union> PFVars_1 p \<union> avoiding_set1) \<Longrightarrow>
   (\<And>t pu p. (t, pu) \<in> set9_T2_pre y2 \<union> set10_T2_pre y2 \<Longrightarrow> U2FVars_1 t (pu p) \<subseteq> FFVars_T21 t \<union> PFVars_1 p \<union> avoiding_set1) \<Longrightarrow>
   U2FVars_1 (T2_ctor (map_T2_pre id id id id id id fst fst fst fst y2)) (U2ctor y2 p) \<subseteq> FFVars_T21 (T2_ctor (map_T2_pre id id id id id id fst fst fst fst y2)) \<union> PFVars_1 p \<union> avoiding_set1"
-  and U2FVars_subset_2: "set6_T2_pre y2 \<inter> (PFVars_2 p \<union> avoiding_set2) = {} \<Longrightarrow>
+  and U2FVars_subset_2: "validP p \<Longrightarrow>
+  pred_T2_pre (\<lambda>_. True) (pred_fun validP validU1 \<circ> snd) (pred_fun validP validU1 \<circ> snd) (pred_fun validP validU2 \<circ> snd) (pred_fun validP validU2 \<circ> snd) y2 \<Longrightarrow>set6_T2_pre y2 \<inter> (PFVars_2 p \<union> avoiding_set2) = {} \<Longrightarrow>
   (\<And>t pu p. (t, pu) \<in> set7_T2_pre y2 \<union> set8_T2_pre y2 \<Longrightarrow> U1FVars_2 t (pu p) \<subseteq> FFVars_T12 t \<union> PFVars_2 p \<union> avoiding_set2) \<Longrightarrow>
   (\<And>t pu p. (t, pu) \<in> set9_T2_pre y2 \<union> set10_T2_pre y2 \<Longrightarrow> U2FVars_2 t (pu p) \<subseteq> FFVars_T22 t \<union> PFVars_2 p \<union> avoiding_set2) \<Longrightarrow>
   U2FVars_2 (T2_ctor (map_T2_pre id id id id id id fst fst fst fst y2)) (U2ctor y2 p) \<subseteq> FFVars_T22 (T2_ctor (map_T2_pre id id id id id id fst fst fst fst y2)) \<union> PFVars_2 p \<union> avoiding_set2"
+  (* closure of validU2 under Umap and Uctor *)
+  and validU2_Umap: "validU2 u2 \<Longrightarrow> bij f1 \<Longrightarrow> |supp (f1::'var::{var_T1_pre,var_T2_pre} \<Rightarrow> 'var)| <o |UNIV::'var set| \<Longrightarrow> bij f2 \<Longrightarrow> |supp (f2::'tyvar::{var_T1_pre,var_T2_pre} \<Rightarrow> 'tyvar)| <o |UNIV::'tyvar set| \<Longrightarrow>
+                     validU2 (U2map f1 f2  (t2::('var, 'tyvar, 'a, 'b) T2) u2)"
+  and validU2_Uctor: "pred_T2_pre (\<lambda>_. True) (pred_fun validP validU1 \<circ> snd) (pred_fun validP validU1 \<circ> snd) (pred_fun validP validU2 \<circ> snd) (pred_fun validP validU2 \<circ> snd) y2
+        \<Longrightarrow> validP p \<Longrightarrow> validU2 (U2ctor y2 p)"
 print_theorems
 
 lemmas U1FVars_subsets = U1FVars_subset_1 U1FVars_subset_2
@@ -815,7 +841,7 @@ lemma U2FVars'_subsets: "set5_T2_pre (y2::(_, _, 'a::{var_T1_pre,var_T2_pre}, 'b
 
 lemma Pmap_imsupp_empty:
   fixes f1::"'var::{var_T1_pre,var_T2_pre} \<Rightarrow> 'var" and f2::"'tyvar::{var_T1_pre,var_T2_pre} \<Rightarrow> 'tyvar"
-  assumes "bij f1" "|supp f1| <o |UNIV::'var set|" "bij f2" "|supp f2| <o |UNIV::'tyvar set|"
+  assumes "validP p" "bij f1" "|supp f1| <o |UNIV::'var set|" "bij f2" "|supp f2| <o |UNIV::'tyvar set|"
     "imsupp f1 \<inter> PFVars_1 p = {}" "imsupp f2 \<inter> PFVars_2 p = {}"
   shows "Pmap f1 f2 p = p"
   apply (rule Pmap_cong_id)
@@ -824,7 +850,7 @@ lemma Pmap_imsupp_empty:
 
 lemma U1ctor_rename:
   fixes f1::"'var::{var_T1_pre,var_T2_pre} \<Rightarrow> 'var" and f2::"'tyvar::{var_T1_pre,var_T2_pre} \<Rightarrow> 'tyvar"
-  assumes "bij f1" "|supp f1| <o |UNIV::'var set|" "bij f2" "|supp f2| <o |UNIV::'tyvar set|"
+  assumes "validP p" "bij f1" "|supp f1| <o |UNIV::'var set|" "bij f2" "|supp f2| <o |UNIV::'tyvar set|"
   shows
     "(\<And>t pu p. (t, pu) \<in> set7_T1_pre y \<union> set8_T1_pre y \<Longrightarrow> U1FVars_1 t (pu p) \<subseteq> FFVars_T11 t \<union> PFVars_1 p \<union> avoiding_set1) \<Longrightarrow>
   (\<And>t pu p. (t, pu) \<in> set9_T1_pre y \<union> set10_T1_pre y \<Longrightarrow> U2FVars_1 t (pu p) \<subseteq> FFVars_T21 t \<union> PFVars_1 p \<union> avoiding_set1) \<Longrightarrow>
@@ -841,7 +867,7 @@ lemma U1ctor_rename:
   apply (rule trans)
    apply (rule trans)
     apply (rule arg_cong2[OF refl, of _ _ U1ctor] arg_cong2[OF refl, of _ _ U2ctor])
-    apply (rule Pmap_imsupp_empty[symmetric, OF assms(1-4)])
+    apply (rule Pmap_imsupp_empty[symmetric, OF assms(1-5)])
      apply ((unfold Int_Un_distrib Un_empty)[1], (erule conjE)+, assumption)+
    apply (unfold PU1map_def PU2map_def)
    apply (rule U1map_Uctor[symmetric] U2map_Uctor[symmetric])
